elf/EncodeRelocElf.v
@@ -64,7 +64,7 @@ Definition encode_section_header (sh: section_header) :=
 Definition encode_section_headers (shs: list section_header) :=
   fold_right (fun sh r => (encode_section_header sh) ++ r) [] shs.
 
-Definition encode_elf_file (ef: elf_file) : (list byte * program) :=
+Definition encode_elf_file (ef: elf_file) : (list byte * program * Globalenvs.Senv.t) :=
   let bs := 
       (encode_elf_header (elf_head ef)) ++
       (encode_sections (elf_sections ef)) ++
@@ -72,4 +72,4 @@ Definition encode_elf_file (ef: elf_file) : (list byte * program) :=
   let p := {| AST.prog_defs   := RelocElf.prog_defs ef;
               AST.prog_public := RelocElf.prog_public ef;
               AST.prog_main   := RelocElf.prog_main ef; |} in
-  (bs, p).
+  (bs, p, prog_senv ef).
